CoqOfRust/std/string.v
@@ -1,6 +1,49 @@
 Require Import CoqOfRust.lib.lib.
 Require Import CoqOfRust.std.convert.
 
+(* ********TYPE DEFS******** *)
+(* 
+[ ] ParseError
+*)
+(* Notation ParseError := Infallible. *)
+
+(* ********STRUCTS******** *)
+(* 
+[x] Drain
+[x] FromUtf8Error
+[x] FromUtf16Error
+[x] String 
+*)
+
+(* pub struct Drain<'a> { /* private fields */ } *)
+Module Drain.
+  Record t : Set := { }.
+End Drain.
+Definition Drain := Drain.t.
+
+(* pub struct FromUtf8Error { /* private fields */ } *)
+Module FromUtf8Error.
+  Record t : Set := { }.
+End FromUtf8Error.
+Definition FromUtf8Error := FromUtf8Error.t.
+
+(* pub struct FromUtf16Error(_); *)
+Module FromUtf16Error.
+  Record t (underscore : Set): Set := { }.
+End FromUtf16Error.
+Definition FromUtf16Error := FromUtf16Error.t.
+
+(* pub struct String { /* private fields */ } *)
+Module String.
+  Definition t : Set := str.
+End String.
+Definition String := String.t.
+
+(* ********TRAITS******** *)
+(* 
+[x] ToString 
+*)
+
 Module ToString.
   Class Trait (Self : Set) : Set := {
     to_string : ref Self -> String;
@@ -17,7 +60,7 @@ Module StringType.
 
   (* The String type (Struct std::string::String) and it's methods  *)
   (* Converts a &str into a String. *)
-  Global Instance FromStr : From str String := {
+  Global Instance FromStr : From.Trait str String := {
     from := from;
   }.
 
