CoqOfRust/std/alloc.v
@@ -1,0 +1,136 @@
+Require Import CoqOfRust.lib.lib.
+
+Require Import CoqOfRust.std.ptr.
+Require Import CoqOfRust.std.result.
+Require Import CoqOfRust.std.marker.
+
+(* *******STRUCTS******** *)
+(* 
+[x] AllocError
+[x] Global
+[x] Layout
+[x] LayoutError
+[x] System
+*)
+
+Module AllocError.
+  Record t : Set := { }.
+End AllocError.
+Definition AllocError := AllocError.t.
+
+Module Global.
+  Record t : Set := { }.
+End Global.
+Definition Global := Global.t.
+
+Module Layout.
+  Record t : Set := { }.
+End Layout.
+Definition Layout := Layout.t.
+
+Module LayoutError.
+  Record t : Set := { }.
+End LayoutError.
+Definition LayoutError := LayoutError.t.
+
+Module System.
+  Record t : Set := { }.
+End System.
+Definition System := System.t.
+
+(* ********TRAITS******** *)
+(* 
+[x] Allocator
+[x] GlobalAlloc
+*)
+
+(* 
+pub unsafe trait Allocator {
+    // ...
+}
+*)
+Module Allocator.
+  Class Trait (Self : Set) : Set := { 
+    (* fn allocate(&self, layout: Layout) -> Result<NonNull<[u8]>, AllocError>; *)
+    allocate : ref Self -> Layout -> Result (NonNull (slice u8)) AllocError;
+    
+    (* unsafe fn deallocate(&self, ptr: NonNull<u8>, layout: Layout); *)
+    deallocate : ref Self -> NonNull u8 -> Layout -> unit;
+
+    (* 
+    fn allocate_zeroed(
+        &self,
+        layout: Layout
+    ) -> Result<NonNull<[u8]>, AllocError> { ... }
+    *)
+    allocate_zeroed : ref Self -> Layout -> Result (NonNull (slice u8)) AllocError;
+
+    (* 
+    unsafe fn grow(
+        &self,
+        ptr: NonNull<u8>,
+        old_layout: Layout,
+        new_layout: Layout
+    ) -> Result<NonNull<[u8]>, AllocError> { ... }
+    *)
+    grow : ref Self -> NonNull u8 -> Layout -> Layout
+         -> Result (NonNull (slice u8)) AllocError;
+
+    (* 
+    unsafe fn grow_zeroed(
+        &self,
+        ptr: NonNull<u8>,
+        old_layout: Layout,
+        new_layout: Layout
+    ) -> Result<NonNull<[u8]>, AllocError> { ... }
+    *)
+    grow_zeroed : ref Self -> NonNull u8 -> Layout -> Layout
+                -> Result (NonNull (slice u8)) AllocError;
+
+    (* 
+    unsafe fn shrink(
+        &self,
+        ptr: NonNull<u8>,
+        old_layout: Layout,
+        new_layout: Layout
+    ) -> Result<NonNull<[u8]>, AllocError> { ... }
+    *)
+    shrink : ref Self -> NonNull u8 -> Layout -> Layout
+            -> Result (NonNull (slice u8)) AllocError;
+
+    (*
+    fn by_ref(&self) -> &Self
+       where Self: Sized { ... }
+    *)
+    by_ref 
+    : ref Self -> ref Self;
+  }.
+End Allocator.
+
+(* 
+pub unsafe trait GlobalAlloc {
+    // Required methods
+    unsafe fn alloc(&self, layout: Layout) -> *mut u8;
+    unsafe fn dealloc(&self, ptr: *mut u8, layout: Layout);
+
+    // Provided methods
+    unsafe fn alloc_zeroed(&self, layout: Layout) -> *mut u8 { ... }
+    unsafe fn realloc(
+        &self,
+        ptr: *mut u8,
+        layout: Layout,
+        new_size: usize
+    ) -> *mut u8 { ... }
+}
+*)
+Module GlobalAlloc.
+  Class Trait (Self : Set) : Set := { 
+    alloc : ref Self -> Layout -> mut_ref u8;
+    dealloc : ref Self -> mut_ref u8 -> Layout -> unit;
+    alloc_zeroed : ref Self -> Layout -> mut_ref u8;
+    realloc : ref Self -> mut_ref u8 -> Layout -> usize -> mut_ref u8;
+  }.
+End GlobalAlloc.
+
+(* ********TYPE DEFINITIONS******** *)
+(* NOTE: Only deprecated defs *)
