CoqOfRust/std/borrow.v
@@ -1,0 +1,87 @@
+Require Import CoqOfRust.lib.lib.
+
+(* ********ENUMS******** *)
+(*
+[?] Cow
+*)
+(* 
+pub enum Cow<'a, B>
+where
+    B: 'a + ToOwned + ?Sized,
+{
+    Borrowed(&'a B),
+    Owned(<B as ToOwned>::Owned),
+}
+*)
+Module Coq.
+  Inductive t (B : Set): Set := 
+  | Borrowed : ref B -> t B
+  (* BUGGED: Cannot define the param *)
+  | Owned : B -> t B
+  .
+End Coq.
+Definition Coq := Coq.t.
+
+
+(* ********TRAITS******** *)
+(*
+[x] Borrow
+[x] BorrowMut
+[x] ToOwned
+*)
+
+(* 
+pub trait Borrow<Borrowed>
+where
+    Borrowed: ?Sized,
+{
+    // Required method
+    fn borrow(&self) -> &Borrowed;
+}
+*)
+Module Borrow.
+  Class Trait (Self Borrowed : Set) : Set := { 
+    borrow : ref Self -> ref Borrowed;
+  }.
+End Borrow.
+
+(* 
+pub trait BorrowMut<Borrowed>: Borrow<Borrowed>
+where
+    Borrowed: ?Sized,
+{
+    // Required method
+    fn borrow_mut(&mut self) -> &mut Borrowed;
+}
+*)
+Module BorrowMut.
+  Class Trait (Self Borrowed : Set) 
+    `{Borrow.Trait Self Borrowed}
+  : Set := { 
+    borrow_mut : mut_ref Self -> mut_ref Borrowed;
+  }.
+End BorrowMut.
+
+(* 
+pub trait ToOwned {
+  type Owned: Borrow<Self>;
+
+  // Required method
+  fn to_owned(&self) -> Self::Owned;
+
+  // Provided method
+  fn clone_into(&self, target: &mut Self::Owned) { ... }
+}
+*)
+Module ToOwned.
+  Class Trait (Self Owned : Set) 
+    `{Borrow.Trait Owned Self}
+  : Set := { 
+    Owned := Owned;
+
+    to_owned : ref Self -> Owned;
+    clone_into : ref Self -> mut_ref Owned;
+  }.
+End ToOwned.
+
+
