CoqOfRust/std/char.v
@@ -1,0 +1,99 @@
+Require Import CoqOfRust.lib.lib.
+(* Require Import CoqOfRust.std.iter. *)
+
+
+(* ********STRUCTS******** *)
+(* 
+[x] CharTryFromError
+[?] DecodeUtf16
+[x] DecodeUtf16Error
+[x] EscapeDebug
+[x] EscapeDefault
+[x] EscapeUnicode
+[x] ParseCharError
+[x] ToLowercase
+[x] ToUppercase
+[x] TryFromCharError
+*)
+
+(* pub struct CharTryFromError(_); *)
+Module CharTryFromError.
+  Record t : Set := { }.
+End CharTryFromError.
+Definition CharTryFromError := CharTryFromError.t.
+
+(* BUGGED: Iterator dependency *)
+(* 
+pub struct DecodeUtf16<I>
+where
+    I: Iterator<Item = u16>,
+{ /* private fields */ }
+*)
+Module DecodeUtf16.
+  Record t (I : Set) : Set := { }.
+End DecodeUtf16.
+Definition DecodeUtf16 := DecodeUtf16.t.
+
+(* pub struct DecodeUtf16Error { /* private fields */ } *)
+Module DecodeUtf16Error.
+  Record t : Set := { }.
+End DecodeUtf16Error.
+Definition DecodeUtf16Error := DecodeUtf16Error.t.
+
+(* pub struct EscapeDebug(_); *)
+Module EscapeDebug.
+  Record t : Set := { }.
+End EscapeDebug.
+Definition EscapeDebug := EscapeDebug.t.
+
+(* pub struct EscapeDefault { /* private fields */ } *)
+Module EscapeDefault.
+  Record t : Set := { }.
+End EscapeDefault.
+Definition EscapeDefault := EscapeDefault.t.
+
+(* pub struct EscapeUnicode { /* private fields */ } *)
+Module EscapeUnicode.
+  Record t : Set := { }.
+End EscapeUnicode.
+Definition EscapeUnicode := EscapeUnicode.t.
+
+(* pub struct ParseCharError { /* private fields */ } *)
+Module ParseCharError.
+  Record t : Set := { }.
+End ParseCharError.
+Definition ParseCharError := ParseCharError.t.
+
+(* pub struct ToLowercase(_); *)
+Module ToLowercase.
+  Record t : Set := { }.
+End ToLowercase.
+Definition ToLowercase := ToLowercase.t.
+
+(* pub struct ToUppercase(_); *)
+Module ToUppercase.
+  Record t : Set := { }.
+End ToUppercase.
+Definition ToUppercase := ToUppercase.t.
+
+(* pub struct TryFromCharError(_); *)
+Module TryFromCharError.
+  Record t : Set := { }.
+End TryFromCharError.
+Definition TryFromCharError := TryFromCharError.t.
+
+(* ********CONSTANTS******** *)
+(* 
+[ ] MAX
+[ ] REPLACEMENT_CHARACTER
+[ ] UNICODE_VERSION
+*)
+
+(* ********FUNCTIONS******** *)
+(* 
+[ ] decode_utf16
+[ ] from_digit
+[ ] from_u32
+[ ] from_u32_unchecked
+*)
+
