CoqOfRust/std/clone.v
@@ -1,0 +1,21 @@
+Require Import CoqOfRust.lib.lib.
+
+(* ********TRAITS******** *)
+(* 
+[x] Clone
+*)
+(* 
+pub trait Clone: Sized {
+    // Required method
+    fn clone(&self) -> Self;
+
+    // Provided method
+    fn clone_from(&mut self, source: &Self) { ... }
+}
+*)
+Module Clone.
+  Class Trait (Self : Set) : Set := {
+    clone : ref Self -> Self;
+    clone_from : mut_ref Self -> ref Self;
+  }.
+End Clone.
