CoqOfRust/std/default.v
@@ -1,0 +1,20 @@
+Require Import CoqOfRust.lib.lib.
+
+Require Import CoqOfRust.std.marker.
+
+(* ********TRAITS******** *)
+(* 
+[x] Default
+*)
+
+(* 
+pub trait Default: Sized {
+    // Required method
+    fn default() -> Self;
+}
+*)
+Module Default.
+  Class Trait (Self : Set) : Set := { 
+    default : Self;
+  }.
+End Default.
