CoqOfRust/std/hint.v
@@ -1,0 +1,11 @@
+Require Import CoqOfRust.lib.lib.
+
+(* NOTE: No traits or structs or enums to be translated *)
+
+(* ********FUNCTIONS******** *)
+(*
+[ ] must_use
+[ ] black_box
+[ ] spin_loop
+[ ] unreachable_unchecked
+*)
