CoqOfRust/std/io.v
@@ -1,0 +1,456 @@
+Require Import CoqOfRust.lib.lib.
+Require Import CoqOfRust.std.fmt.
+
+
+(* ********STRUCTS******** *)
+(* 
+[x] BorrowedBuf
+[x] BorrowedCursor
+[x] BufReader
+[x] BufWriter
+[x] Bytes
+[x] Chain
+[x] Cursor
+[x] Empty
+[x] Error
+[x] IntoInnerError
+[x] IoSlice
+[x] IoSliceMut
+[x] LineWriter
+[x] Lines
+[x] Repeat
+[x] Sink
+[x] Split
+[x] Stderr
+[x] StderrLock
+[x] Stdin
+[x] StdinLock
+[x] Stdout
+[x] StdoutLock
+[x] Take
+[x] WriterPanicked
+*)
+
+(* pub struct BorrowedBuf<'data> { /* private fields */ } *)
+Module BorrowedBuf.
+  Record t : Set := { }.
+End BorrowedBuf.
+Definition BorrowedBuf := BorrowedBuf.t.
+
+(* pub struct BorrowedCursor<'a> { /* private fields */ } *)
+Module BorrowedCursor.
+  Record t : Set := { }.
+End BorrowedCursor.
+Definition BorrowedCursor := BorrowedCursor.t.
+
+(* pub struct BufReader<R> { /* private fields */ } *)
+Module BufReader.
+  Record t (R : Set) : Set := { }.
+End BufReader.
+Definition BufReader := BufReader.t.
+
+(* pub struct IoSlice<'a>(_); *)
+Module IoSlice.
+  Record t : Set := { }.
+End IoSlice.
+Definition IoSlice := IoSlice.t.
+
+(* 
+pub trait Write {
+    // Required methods
+    fn write(&mut self, buf: &[u8]) -> Result<usize>;
+    fn flush(&mut self) -> Result<()>;
+
+    // Provided methods
+    fn write_vectored(&mut self, bufs: &[IoSlice<'_>]) -> Result<usize> { ... }
+    fn is_write_vectored(&self) -> bool { ... }
+    fn write_all(&mut self, buf: &[u8]) -> Result<()> { ... }
+    fn write_all_vectored(&mut self, bufs: &mut [IoSlice<'_>]) -> Result<()> { ... }
+    fn write_fmt(&mut self, fmt: Arguments<'_>) -> Result<()> { ... }
+    fn by_ref(&mut self) -> &mut Self
+       where Self: Sized { ... }
+}
+*)
+Module Write.
+  Class Trait (Self : Set) : Set := { 
+    write : mut_ref Self -> ref (slice u8) -> Result usize;
+    flush : mut_ref Self -> Result unit;
+    write_vectored : mut_ref Self -> ref (slice IoSlice) -> Result usize;
+    is_write_vectored : mut_ref Self -> bool;
+    write_all : mut_ref Self -> ref (slice u8) -> Result unit;
+    write_all_vectored : mut_ref Self -> mut_ref (slice IoSlice) -> Result unit;
+    write_fmt : mut_ref Self -> Arguments -> Result unit;
+    by_ref : mut_ref Self -> mut_ref Self;
+  }.
+End Write.
+
+
+(* pub struct BufWriter<W: Write> { /* private fields */ } *)
+Module BufWriter.
+  Record t (W : Set) `{Write.Trait W} : Set := { }.
+End BufWriter.
+Definition BufWriter := BufWriter.t.
+
+(* pub struct Bytes<R> { /* private fields */ } *)
+Module Bytes.
+  Record t (R : Set) : Set := { }.
+End Bytes.
+Definition Bytes := Bytes.t.
+
+(* pub struct Chain<T, U> { /* private fields */ } *)
+Module Chain.
+  Record t (T U : Set) : Set := { }.
+End Chain.
+Definition Chain := Chain.t.
+
+(* pub struct Cursor<T> { /* private fields */ } *)
+Module Cursor.
+  Record t (T : Set) : Set := { }.
+End Cursor.
+Definition Cursor := Cursor.t.
+
+(* pub struct Empty; *)
+Module Empty.
+  Record t : Set := { }.
+End Empty.
+Definition Empty := Empty.t.
+
+(* pub struct Error { /* private fields */ } *)
+Module Error.
+  Record t : Set := { }.
+End Error.
+Definition Error := Error.t.
+
+(* pub struct IntoInnerError<W>(_, _); *)
+Module IntoInnerError.
+  Record t (W : Set) : Set := { }.
+End IntoInnerError.
+Definition IntoInnerError := IntoInnerError.t.
+
+(* pub struct IoSliceMut<'a>(_); *)
+Module IoSliceMut.
+  Record t : Set := { }.
+End IoSliceMut.
+Definition IoSliceMut := IoSliceMut.t.
+
+(* pub struct LineWriter<W: Write> { /* private fields */ } *)
+Module LineWriter.
+  Record t (W : Set) `{Write.Trait W} : Set := { }.
+End LineWriter.
+Definition LineWriter := LineWriter.t.
+
+(* pub struct Lines<B> { /* private fields */ } *)
+Module Lines.
+  Record t (B : Set) : Set := { }.
+End Lines.
+Definition Lines := Lines.t.
+
+(* pub struct Repeat { /* private fields */ } *)
+Module Repeat.
+  Record t : Set := { }.
+End Repeat.
+Definition Repeat := Repeat.t.
+
+(* pub struct Sink; *)
+Module Sink.
+  Record t : Set := { }.
+End Sink.
+Definition Sink := Sink.t.
+
+(* pub struct Split<B> { /* private fields */ } *)
+Module Split.
+  Record t (B : Set) : Set := { }.
+End Split.
+Definition Split := Split.t.
+
+(* pub struct Stderr { /* private fields */ } *)
+Module Stderr.
+  Record t : Set := { }.
+End Stderr.
+Definition Stderr := Stderr.t.
+
+(* pub struct StderrLock<'a> { /* private fields */ } *)
+Module StderrLock.
+  Record t : Set := { }.
+End StderrLock.
+Definition StderrLock := StderrLock.t.
+
+(* pub struct Stdin { /* private fields */ } *)
+Module Stdin.
+  Record t : Set := { }.
+End Stdin.
+Definition Stdin := Stdin.t.
+
+(* pub struct StdinLock<'a> { /* private fields */ } *)
+Module StdinLock.
+  Record t : Set := { }.
+End StdinLock.
+Definition StdinLock := StdinLock.t.
+
+(* pub struct Stdout { /* private fields */ } *)
+Module Stdout.
+  Record t : Set := { }.
+End Stdout.
+Definition Stdout := Stdout.t.
+
+(* pub struct StdoutLock<'a> { /* private fields */ } *)
+Module StdoutLock.
+  Record t : Set := { }.
+End StdoutLock.
+Definition StdoutLock := StdoutLock.t.
+
+(* pub struct Take<T> { /* private fields */ } *)
+Module Take.
+  Record t (T : Set) : Set := { }.
+End Take.
+Definition Take := Take.t.
+
+(* pub struct WriterPanicked { /* private fields */ } *)
+Module WriterPanicked.
+  Record t : Set := { }.
+End WriterPanicked.
+Definition WriterPanicked := WriterPanicked.t.
+
+
+
+
+(* ********ENUMS******** *)
+
+(* 
+[x] ErrorKind
+[x] SeekFrom
+*)
+
+(* 
+pub enum ErrorKind {
+    NotFound,
+    PermissionDenied,
+    ConnectionRefused,
+    ConnectionReset,
+    HostUnreachable,
+    NetworkUnreachable,
+    ConnectionAborted,
+    NotConnected,
+    AddrInUse,
+    AddrNotAvailable,
+    NetworkDown,
+    BrokenPipe,
+    AlreadyExists,
+    WouldBlock,
+    NotADirectory,
+    IsADirectory,
+    DirectoryNotEmpty,
+    ReadOnlyFilesystem,
+    FilesystemLoop,
+    StaleNetworkFileHandle,
+    InvalidInput,
+    InvalidData,
+    TimedOut,
+    WriteZero,
+    StorageFull,
+    NotSeekable,
+    FilesystemQuotaExceeded,
+    FileTooLarge,
+    ResourceBusy,
+    ExecutableFileBusy,
+    Deadlock,
+    CrossesDevices,
+    TooManyLinks,
+    InvalidFilename,
+    ArgumentListTooLong,
+    Interrupted,
+    Unsupported,
+    UnexpectedEof,
+    OutOfMemory,
+    Other,
+    // some variants omitted
+}
+*)
+Module ErrorKind.
+  Inductive t :=
+  | NotFound
+  | PermissionDenied
+  | ConnectionRefused
+  | ConnectionReset
+  | HostUnreachable
+  | NetworkUnreachable
+  | ConnectionAborted
+  | NotConnected
+  | AddrInUse
+  | AddrNotAvailable
+  | NetworkDown
+  | BrokenPipe
+  | AlreadyExists
+  | WouldBlock
+  | NotADirectory
+  | IsADirectory
+  | DirectoryNotEmpty
+  | ReadOnlyFilesystem
+  | FilesystemLoop
+  | StaleNetworkFileHandle
+  | InvalidInput
+  | InvalidData
+  | TimedOut
+  | WriteZero
+  | StorageFull
+  | NotSeekable
+  | FilesystemQuotaExceeded
+  | FileTooLarge
+  | ResourceBusy
+  | ExecutableFileBusy
+  | Deadlock
+  | CrossesDevices
+  | TooManyLinks
+  | InvalidFilename
+  | ArgumentListTooLong
+  | Interrupted
+  | Unsupported
+  | UnexpectedEof
+  | OutOfMemory
+  | Other
+  .
+End ErrorKind.
+Definition ErrorKind := ErrorKind.t.
+
+(* 
+pub enum SeekFrom {
+    Start(u64),
+    End(i64),
+    Current(i64),
+}
+*)
+Module SeekFrom.
+  Inductive t : Set :=
+  | Start : u64 -> t
+  | End : i64 -> t
+  | Current : i64 -> t
+  .
+End SeekFrom.
+Definition SeekFrom := SeekFrom.t.
+
+(* ********TRAITS******** *)
+(* 
+[x]IsTerminal
+[x]BufRead
+[x]Read
+[ ]Seek
+[ ]Write 
+*)
+
+(* 
+pub trait IsTerminal: Sealed {
+    // Required method
+    fn is_terminal(&self) -> bool;
+}
+*)
+Module IsTerminal.
+  Class Trait (Self : Set) : Set := { 
+    is_terminal : ref Self -> bool;
+  }.
+End IsTerminal.
+
+(* 
+pub trait Read {
+    // Required method
+    fn read(&mut self, buf: &mut [u8]) -> Result<usize>;
+
+    // Provided methods
+    fn read_vectored(&mut self, bufs: &mut [IoSliceMut<'_>]) -> Result<usize> { ... }
+    fn is_read_vectored(&self) -> bool { ... }
+    fn read_to_end(&mut self, buf: &mut Vec<u8>) -> Result<usize> { ... }
+    fn read_to_string(&mut self, buf: &mut String) -> Result<usize> { ... }
+    fn read_exact(&mut self, buf: &mut [u8]) -> Result<()> { ... }
+    fn read_buf(&mut self, buf: BorrowedCursor<'_>) -> Result<()> { ... }
+    fn read_buf_exact(&mut self, cursor: BorrowedCursor<'_>) -> Result<()> { ... }
+    fn by_ref(&mut self) -> &mut Self
+       where Self: Sized { ... }
+    fn bytes(self) -> Bytes<Self> ⓘ
+       where Self: Sized { ... }
+    fn chain<R: Read>(self, next: R) -> Chain<Self, R> ⓘ
+       where Self: Sized { ... }
+    fn take(self, limit: u64) -> Take<Self> ⓘ
+       where Self: Sized { ... }
+}
+*)
+Module Read.
+  Class Trait (Self : Set) : Set := { 
+    read : mut_ref Self -> mut_ref (slice u8) -> Result usize;
+    read_vectored : mut_ref Self -> mut_ref (slice IoSliceMut) -> Result usize;
+    is_read_vectored : ref Self -> bool;
+    read_to_end : mut_ref Self -> mut_ref (slice u8) -> Result usize;
+    read_to_string : mut_ref Self -> mut_ref Steing -> Result usize;
+    read_exact : mut_ref Self -> mut_ref (slice u8) -> Result unit;
+    read_buf : mut_ref Self -> BorrowedCursor -> Result unit;
+    read_buf_exact : mut_ref Self -> BorrowedCursor -> Result unit;
+    by_ref : mut_ref Self -> mut_ref Self;
+    bytes : Self -> Bytes Self;
+    chain (R : Read) : Self -> R -> Chain Self R;
+    take : Self -> u64 -> Take Self;
+  }.
+End Read.
+
+(* 
+pub trait BufRead: Read {
+    // Required methods
+    fn fill_buf(&mut self) -> Result<&[u8]>;
+    fn consume(&mut self, amt: usize);
+
+    // Provided methods
+    fn has_data_left(&mut self) -> Result<bool> { ... }
+    fn read_until(&mut self, byte: u8, buf: &mut Vec<u8>) -> Result<usize> { ... }
+    fn read_line(&mut self, buf: &mut String) -> Result<usize> { ... }
+    fn split(self, byte: u8) -> Split<Self>
+       where Self: Sized { ... }
+    fn lines(self) -> Lines<Self>
+       where Self: Sized { ... }
+}
+*)
+Module BufRead.
+  Class Trait (Self : Set) `{Read.Trait Self}: Set := { 
+    fill_buf : mut_ref Self -> Result (ref (slice u8));
+    consume : mut_ref Self -> usize -> unit;
+    has_data_left : mut_ref Self -> Result bool;
+    read_until : mut_ref Self -> u8 -> mut_ref (Vec u8) -> Result usize;
+    read_line : mut_ref Self -> mut_ref String -> Result usize;
+    split : Self -> u8 -> Split Self;
+    lines : mut_ref Self -> Lines Self;
+  }.
+End BufRead.
+
+(* 
+pub trait Seek {
+    // Required method
+    fn seek(&mut self, pos: SeekFrom) -> Result<u64>;
+
+    // Provided methods
+    fn rewind(&mut self) -> Result<()> { ... }
+    fn stream_len(&mut self) -> Result<u64> { ... }
+    fn stream_position(&mut self) -> Result<u64> { ... }
+}
+*)
+Module Seek.
+  Class Trait (Self : Set) : Set := { 
+    seek : mut_ref Self -> SeekFrom -> Result u64;
+    rewind : mut_ref Self -> Result unit;
+    stream_len : mut_ref Self -> Result u64;
+    stream_position : mut_ref Self -> Result u64;
+  }.
+End Seek.
+
+(* ********FUNCTIONS******** *)
+(*
+[ ] copy
+[ ] empty
+[ ] read_to_string
+[ ] repeat
+[ ] sink
+[ ] stderr
+[ ] stdin
+[ ] stdout
+*)
+
+(* ********TYPE DEFINITIONS******** *)
+(*
+[ ] RawOsError
+[ ] Result
+*)
