CoqOfRust/std/path.v
@@ -1,0 +1,124 @@
+Require Import CoqOfRust.lib.lib.
+
+Require Import CoqOfRust.std.ffi.
+
+(* ********STRUCTS******** *)
+(*
+[x] Ancestors
+[x] Components
+[x] Display
+[x] Iter
+[x] Path
+[x] PathBuf
+[x] PrefixComponent
+[x] StripPrefixError
+*)
+
+(* pub struct Ancestors<'a> { /* private fields */ } *)
+Module Ancestors.
+  Record t : Set := { }.
+End Ancestors.
+Definition Ancestors := Ancestors.t.
+
+(* pub struct Components<'a> { /* private fields */ } *)
+Module Components.
+  Record t : Set := { }.
+End Components.
+Definition Components := Components.t.
+
+(* pub struct Display<'a> { /* private fields */ } *)
+Module Display.
+  Record t : Set := { }.
+End Display.
+Definition Display := Display.t.
+
+(* pub struct Iter<'a> { /* private fields */ } *)
+Module Iter.
+  Record t : Set := { }.
+End Iter.
+Definition Iter := Iter.t.
+
+(* pub struct Path { /* private fields */ } *)
+Module Path.
+  Record t : Set := { }.
+End Path.
+Definition Path := Path.t.
+
+(* pub struct PathBuf { /* private fields */ } *)
+Module PathBuf.
+  Record t : Set := { }.
+End PathBuf.
+Definition PathBuf := PathBuf.t.
+
+(* pub struct PrefixComponent<'a> { /* private fields */ } *)
+Module PrefixComponent.
+  Record t : Set := { }.
+End PrefixComponent.
+Definition PrefixComponent := PrefixComponent.t.
+
+(* pub struct StripPrefixError(_); *)
+Module StripPrefixError.
+  Record t : Set := { }.
+End StripPrefixError.
+Definition StripPrefixError := StripPrefixError.t.
+
+
+(* ********ENUMS******** *)
+(*
+[x] Component
+[x] Prefix
+*)
+
+(* 
+pub enum Component<'a> {
+    Prefix(PrefixComponent<'a>),
+    RootDir,
+    CurDir,
+    ParentDir,
+    Normal(&'a OsStr),
+}
+*)
+Module Component.
+  Inductive t : Set := 
+  | Prefix : PrefixComponent -> t
+  | RootDir : t
+  | CurDir : t
+  | ParentDir : t
+  | Normal : ref OsStr -> t
+  .
+End Component.
+Definition Component := Component.t.
+
+(* 
+pub enum Prefix<'a> {
+    Verbatim(&'a OsStr),
+    VerbatimUNC(&'a OsStr, &'a OsStr),
+    VerbatimDisk(u8),
+    DeviceNS(&'a OsStr),
+    UNC(&'a OsStr, &'a OsStr),
+    Disk(u8),
+}
+*)
+Module Prefix.
+  Inductive t : Set := 
+  | Verbatim : ref OsStr -> t
+  | VerbatimUNC : ref OsStr -> ref OsStr -> t
+  | VerbatimDisk : u8 -> t
+  | DeviceNS : ref OsStr -> t
+  | UNC : ref OsStr -> ref OsStr -> t
+  | Disk : u8 -> t
+  .
+End Prefix.
+Definition Prefix := Prefix.t.
+
+(* ********CONSTANTS******** *)
+(*
+[ ] MAIN_SEPARATOR
+[ ] MAIN_SEPARATOR_STR
+*)
+
+(* ********FUNCTIONS******** *)
+(*
+[ ] absolute
+[ ] is_separator
+*)
