CoqOfRust/std/pin.v
@@ -1,0 +1,8 @@
+Require Import CoqOfRust.lib.lib.
+
+(* ********STRUCTS******** *)
+(* pub struct Pin<P> { /* private fields */ } *)
+Module Pin.
+  Record t (P : Set) : Set := { }.
+End Pin.
+Definition Pin := Pin.t.
