CoqOfRust/std/rc.v
@@ -1,0 +1,28 @@
+Require Import CoqOfRust.lib.lib.
+
+(* ********STRUCTS******** *)
+(*
+[x] Rc
+[x] Weak
+*)
+(* 
+pub struct Rc<T>
+where
+    T: ?Sized,
+{ /* private fields */ }
+*)
+Module Rc.
+  Record t (T : Set) : Set := { }.
+End Rc.
+Definition Rc := Rc.t.
+
+(* 
+pub struct Weak<T>
+where
+    T: ?Sized,
+{ /* private fields */ }
+*)
+Module Weak.
+  Record t (T : Set) : Set := { }.
+End Weak.
+Definition Weak := Weak.t.
