CoqOfRust/std/time.v
@@ -1,0 +1,45 @@
+Require Import CoqOfRust.lib.lib.
+
+(* ********STRUCTS******** *)
+(* 
+[x] Duration
+[x] Instant
+[x] SystemTime
+[x] SystemTimeError
+[x] TryFromFloatSecsError
+*)
+
+(* pub struct Duration { /* private fields */ } *)
+Module Duration.
+  Record t : Set := { }.
+End Duration.
+Definition Duration := Duration.t.
+
+(* pub struct Instant(_); *)
+Module Instant.
+  Record t : Set := { }.
+End Instant.
+Definition Instant := Instant.t.
+
+(* pub struct SystemTime(_); *)
+Module SystemTime.
+  Record t : Set := { }.
+End SystemTime.
+Definition SystemTime := SystemTime.t.
+
+(* pub struct SystemTimeError(_); *)
+Module SystemTimeError.
+  Record t : Set := { }.
+End SystemTimeError.
+Definition SystemTimeError := SystemTimeError.t.
+
+(* pub struct TryFromFloatSecsError { /* private fields */ } *)
+Module TryFromFloatSecsError.
+  Record t : Set := { }.
+End TryFromFloatSecsError.
+Definition TryFromFloatSecsError := TryFromFloatSecsError.t.
+
+(* ********CONSTANTS******** *)
+(* 
+[ ] UNIX_EPOCH
+*)
